theories/Events/MapDefault.v
@@ -73,7 +73,7 @@ Section Map.
   *)
   (* Definition interp_map {E d} : itree (mapE d +' E) ~> stateT map (itree E) := *)
     (* interp_state (case_ handle_map pure_state). *)
-  Definition interp_map {E d F} `{View (mapE d) F (stateT map (itree E))}
+  Definition interp_map {E d F} `{Subevent (mapE d) F} `{Trigger F (stateT map (itree E))}
     : itree (mapE d +' E) ~> stateT map (itree E) :=
             interp_state (over' handle_map).
 
