theories/Events/State.v
@@ -59,13 +59,17 @@ Section State.
     := fun _ e s => Vis e (fun x => Ret (s, x)).
   *)
 
-  Definition run_state {E F} `{View stateE F (stateT S (itree E))}
+  Definition run_state {E F} `{Subevent stateE F} `{Trigger F (stateT S (itree E))}
     : itree F ~> stateT S (itree E)
     := interp_state (over' handle_state).
 
   Definition run_state' {E F} `{Subevent stateE F} `{Trigger F (stateT S (itree E))}
     : itree F ~> stateT S (itree E)
     := interp_state (over handle_state).
+
+  Definition run_state' {E F} `{View stateE F (stateT S (itree E))}
+    : itree F ~> stateT S (itree E)
+    := interp_state (over' handle_state).
 
 End State.
 
